src/MicroSail/SmallStep/Step.v
@@ -46,89 +46,95 @@ Module SmallStep
   Import CtxNotations.
   Import EnvNotations.
 
-  Inductive Step {Γ : Ctx (𝑿 * Ty)} : forall {σ : Ty} (γ1 γ2 : RegStore) (μ1 μ2 : Memory) (δ1 δ2 : LocalStore Γ) (s1 s2 : Stm Γ σ), Prop :=
+  Inductive Step {Γ : Ctx (𝑿 * Ty)} {τ : Ty} (γ : RegStore) (μ : Memory) (δ : LocalStore Γ) :
+    forall (γ2 : RegStore) (μ2 : Memory) (δ2 : LocalStore Γ) (s1 s2 : Stm Γ τ), Prop :=
 
   | step_stm_exp
-      (γ : RegStore) (μ : Memory) (δ : LocalStore Γ) (σ : Ty) (e : Exp Γ σ) :
-      ⟨ γ , μ , δ , (stm_exp e) ⟩ ---> ⟨ γ , μ , δ , stm_lit σ (eval e δ) ⟩
+      (e : Exp Γ τ) :
+      ⟨ γ , μ , δ , (stm_exp e) ⟩ ---> ⟨ γ , μ , δ , stm_lit τ (eval e δ) ⟩
 
   | step_stm_let_value
-      (γ : RegStore) (μ : Memory) (δ : LocalStore Γ) (x : 𝑿) (τ σ : Ty) (v : Lit τ) (k : Stm (Γ ▻ (x , τ)) σ) :
-      ⟨ γ , μ , δ , stm_let x τ (stm_lit τ v) k ⟩ ---> ⟨ γ , μ , δ , stm_block (env_snoc env_nil (x,τ) v) k ⟩
+      (x : 𝑿) (σ : Ty) (v : Lit σ) (k : Stm (Γ ▻ (x,σ)) τ) :
+      ⟨ γ , μ , δ , stm_let x σ (stm_lit σ v) k ⟩ ---> ⟨ γ , μ , δ , stm_block (env_snoc env_nil (x,σ) v) k ⟩
   | step_stm_let_fail
-      (γ : RegStore) (μ : Memory) (δ : LocalStore Γ) (x : 𝑿) (τ σ : Ty) (s : string) (k : Stm (Γ ▻ (x , τ)) σ) :
-      ⟨ γ , μ , δ, stm_let x τ (stm_fail τ s) k ⟩ ---> ⟨ γ , μ , δ , stm_fail σ s ⟩
+      (x : 𝑿) (σ : Ty) (s : string) (k : Stm (Γ ▻ (x,σ)) τ) :
+      ⟨ γ , μ , δ, stm_let x σ (stm_fail σ s) k ⟩ ---> ⟨ γ , μ , δ , stm_fail τ s ⟩
   | step_stm_let_step
-      (γ γ' : RegStore) (μ μ' : Memory) (δ δ' : LocalStore Γ) (x : 𝑿) (τ σ : Ty)
-      (s : Stm Γ τ) (s' : Stm Γ τ) (k : Stm (Γ ▻ (x , τ)) σ) :
+      (x : 𝑿) (σ : Ty) (s s' : Stm Γ σ) (k : Stm (Γ ▻ (x,σ)) τ)
+      (γ' : RegStore) (μ' : Memory) (δ' : LocalStore Γ) :
       ⟨ γ , μ , δ , s ⟩ ---> ⟨ γ' , μ' , δ' , s' ⟩ ->
-      ⟨ γ , μ , δ , stm_let x τ s k ⟩ ---> ⟨ γ', μ' , δ' , stm_let x τ s' k ⟩
+      ⟨ γ , μ , δ , stm_let x σ s k ⟩ ---> ⟨ γ', μ' , δ' , stm_let x σ s' k ⟩
   | step_stm_block_value
-      (γ : RegStore) (μ : Memory) (δ : LocalStore Γ) (Δ : Ctx (𝑿 * Ty)) (δΔ : LocalStore Δ) (σ : Ty) (v : Lit σ) :
-      ⟨ γ , μ , δ , stm_block δΔ (stm_lit σ v) ⟩ ---> ⟨ γ , μ , δ , stm_lit σ v ⟩
+      (Δ : Ctx (𝑿 * Ty)) (δΔ : LocalStore Δ) (v : Lit τ) :
+      ⟨ γ , μ , δ , stm_block δΔ (stm_lit τ v) ⟩ ---> ⟨ γ , μ , δ , stm_lit τ v ⟩
   | step_stm_block_fail
-      (γ : RegStore) (μ : Memory) (δ : LocalStore Γ) (Δ : Ctx (𝑿 * Ty)) (δΔ : LocalStore Δ) (σ : Ty) (s : string) :
-      ⟨ γ , μ , δ , stm_block δΔ (stm_fail σ s) ⟩ ---> ⟨ γ , μ , δ , stm_fail σ s ⟩
+      (Δ : Ctx (𝑿 * Ty)) (δΔ : LocalStore Δ) (s : string) :
+      ⟨ γ , μ , δ , stm_block δΔ (stm_fail τ s) ⟩ ---> ⟨ γ , μ , δ , stm_fail τ s ⟩
   | step_stm_block_step
-      (γ γ' : RegStore) (μ μ' : Memory) (δ δ' : LocalStore Γ) (Δ : Ctx (𝑿 * Ty)) (δΔ δΔ' : LocalStore Δ) (σ : Ty) (k k' : Stm (Γ ▻▻ Δ) σ) :
+      (Δ : Ctx (𝑿 * Ty)) (δΔ δΔ' : LocalStore Δ) (k k' : Stm (Γ ▻▻ Δ) τ)
+      (γ' : RegStore) (μ' : Memory) (δ' : LocalStore Γ) :
       ⟨ γ , μ , δ ►► δΔ , k ⟩ ---> ⟨ γ', μ' , δ' ►► δΔ' , k' ⟩ ->
       ⟨ γ , μ , δ , stm_block δΔ k ⟩ ---> ⟨ γ' , μ' , δ' , stm_block δΔ' k' ⟩
 
   | step_stm_seq_step
-      (γ γ' : RegStore) (μ μ' : Memory) (δ δ' : LocalStore Γ) (τ σ : Ty) (s s' : Stm Γ τ) (k : Stm Γ σ) :
+      (σ : Ty) (s s' : Stm Γ σ) (k : Stm Γ τ)
+      (γ' : RegStore) (μ' : Memory) (δ' : LocalStore Γ) :
       ⟨ γ , μ , δ , s ⟩ ---> ⟨ γ' , μ' , δ' , s' ⟩ ->
       ⟨ γ , μ , δ , stm_seq s k ⟩ ---> ⟨ γ' , μ' , δ' , stm_seq s' k ⟩
   | step_stm_seq_value
-      (γ : RegStore) (μ : Memory) (δ : LocalStore Γ) (τ σ : Ty) (v : Lit τ) (k : Stm Γ σ) :
-      ⟨ γ , μ , δ , stm_seq (stm_lit τ v) k ⟩ ---> ⟨ γ , μ , δ , k ⟩
+      (σ : Ty) (v : Lit σ) (k : Stm Γ τ) :
+      ⟨ γ , μ , δ , stm_seq (stm_lit σ v) k ⟩ ---> ⟨ γ , μ , δ , k ⟩
   | step_stm_seq_fail
-      (γ : RegStore) (μ : Memory) (δ : LocalStore Γ) (τ σ : Ty) (s : string) (k : Stm Γ σ) :
-      ⟨ γ , μ , δ , stm_seq (stm_fail τ s) k ⟩ ---> ⟨ γ , μ , δ , stm_fail σ s ⟩
+      (σ : Ty) (s : string) (k : Stm Γ τ) :
+      ⟨ γ , μ , δ , stm_seq (stm_fail σ s) k ⟩ ---> ⟨ γ , μ , δ , stm_fail τ s ⟩
 
   | step_stm_call
-      (γ : RegStore) (μ : Memory) (δ : LocalStore Γ) {σs σ} {f : 𝑭 σs σ} (es : NamedEnv (Exp Γ) σs) :
+      {Δ} {f : 𝑭 Δ τ} (es : NamedEnv (Exp Γ) Δ) :
       ⟨ γ , μ , δ , stm_call f es ⟩ --->
-      ⟨ γ , μ , δ , stm_call_frame σs (evals es δ) σ (Pi f) ⟩
+      ⟨ γ , μ , δ , stm_call_frame (evals es δ) (Pi f) ⟩
   | step_stm_call_frame_step
-      (γ γ' : RegStore) (μ μ' : Memory) (δ : LocalStore Γ) (Δ : Ctx (𝑿 * Ty)) {δΔ δΔ' : LocalStore Δ} (τ : Ty)
-      (s s' : Stm Δ τ) :
+      (Δ : Ctx (𝑿 * Ty)) {δΔ δΔ' : LocalStore Δ} (s s' : Stm Δ τ)
+      (γ' : RegStore) (μ' : Memory) :
       ⟨ γ , μ , δΔ , s ⟩ ---> ⟨ γ' , μ' , δΔ' , s' ⟩ ->
-      ⟨ γ , μ , δ , stm_call_frame Δ δΔ τ s ⟩ ---> ⟨ γ' , μ' , δ , stm_call_frame Δ δΔ' τ s' ⟩
+      ⟨ γ , μ , δ , stm_call_frame δΔ s ⟩ ---> ⟨ γ' , μ' , δ , stm_call_frame δΔ' s' ⟩
   | step_stm_call_frame_value
-      (γ : RegStore) (μ : Memory) (δ : LocalStore Γ) (Δ : Ctx (𝑿 * Ty)) {δΔ : LocalStore Δ} (τ : Ty) (v : Lit τ) :
-      ⟨ γ , μ , δ , stm_call_frame Δ δΔ τ (stm_lit τ v) ⟩ ---> ⟨ γ , μ , δ , stm_lit τ v ⟩
+      (Δ : Ctx (𝑿 * Ty)) {δΔ : LocalStore Δ} (v : Lit τ) :
+      ⟨ γ , μ , δ , stm_call_frame δΔ (stm_lit τ v) ⟩ ---> ⟨ γ , μ , δ , stm_lit τ v ⟩
   | step_stm_call_frame_fail
-      (γ : RegStore) (μ : Memory) (δ : LocalStore Γ) (Δ : Ctx (𝑿 * Ty)) {δΔ : LocalStore Δ} (τ : Ty) (s : string) :
-      ⟨ γ , μ , δ , stm_call_frame Δ δΔ τ (stm_fail τ s) ⟩ ---> ⟨ γ , μ , δ , stm_fail τ s ⟩
+      (Δ : Ctx (𝑿 * Ty)) {δΔ : LocalStore Δ} (s : string) :
+      ⟨ γ , μ , δ , stm_call_frame δΔ (stm_fail τ s) ⟩ ---> ⟨ γ , μ , δ , stm_fail τ s ⟩
   | step_stm_call_external
-      (γ γ' : RegStore) (μ μ' : Memory) (δ : LocalStore Γ) {σs σ} {f : 𝑭𝑿 σs σ} (es : NamedEnv (Exp Γ) σs) (res : string + Lit σ) :
+      {Δ} {f : 𝑭𝑿 Δ τ} (es : NamedEnv (Exp Γ) Δ) (res : string + Lit τ)
+      (γ' : RegStore) (μ' : Memory) :
       ExternalCall f (evals es δ) res γ γ' μ μ' ->
       ⟨ γ  , μ  , δ , stm_call_external f es ⟩ --->
       ⟨ γ' , μ' , δ , match res with
-                      | inl msg => stm_fail σ msg
-                      | inr v__σ  => stm_lit σ v__σ
+                      | inl msg => stm_fail τ msg
+                      | inr v__σ  => stm_lit τ v__σ
                       end ⟩
 
   | step_stm_assign_value
-      (γ : RegStore) (μ : Memory) (δ : LocalStore Γ) (x : 𝑿) (σ : Ty) {xInΓ : InCtx (x , σ) Γ} (v : Lit σ) :
-      ⟨ γ , μ , δ , stm_assign x (stm_lit σ v) ⟩ ---> ⟨ γ , μ , δ ⟪ x ↦ v ⟫ , stm_lit σ v ⟩
+      (x : 𝑿) {xInΓ : InCtx (x,τ) Γ} (v : Lit τ) :
+      ⟨ γ , μ , δ , stm_assign x (stm_lit τ v) ⟩ ---> ⟨ γ , μ , δ ⟪ x ↦ v ⟫ , stm_lit τ v ⟩
   | step_stm_assign_fail
-      (γ : RegStore) (μ : Memory) (δ : LocalStore Γ) (x : 𝑿) (σ : Ty) {xInΓ : InCtx (x , σ) Γ} (s : string) :
-      ⟨ γ , μ , δ , stm_assign x (stm_fail σ s) ⟩ ---> ⟨ γ , μ , δ , stm_fail σ s ⟩
+      (x : 𝑿) {xInΓ : InCtx (x,τ) Γ} (s : string) :
+      ⟨ γ , μ , δ , stm_assign x (stm_fail τ s) ⟩ ---> ⟨ γ , μ , δ , stm_fail τ s ⟩
   | step_stm_assign_step
-      (γ γ' : RegStore) (μ μ' : Memory) (δ δ' : LocalStore Γ) (x : 𝑿) (σ : Ty) {xInΓ : InCtx (x , σ) Γ} (s s' : Stm Γ σ) :
+      (x : 𝑿) {xInΓ : InCtx (x,τ) Γ} (s s' : Stm Γ τ)
+      (γ' : RegStore) (μ' : Memory) (δ' : LocalStore Γ) :
       ⟨ γ , μ , δ , s ⟩ ---> ⟨ γ' , μ' , δ' , s' ⟩ ->
       ⟨ γ , μ , δ , stm_assign x s ⟩ ---> ⟨ γ' , μ' , δ' , stm_assign x s' ⟩
 
   | step_stm_if
-      (γ : RegStore) (μ : Memory) (δ : LocalStore Γ) (e : Exp Γ ty_bool) (σ : Ty) (s1 s2 : Stm Γ σ) :
+      (e : Exp Γ ty_bool) (s1 s2 : Stm Γ τ) :
       ⟨ γ , μ , δ , stm_if e s1 s2 ⟩ ---> ⟨ γ , μ , δ , if eval e δ then s1 else s2 ⟩
-  | step_stm_assert
-      (γ : RegStore) (μ : Memory) (δ : LocalStore Γ) (e1 : Exp Γ ty_bool) (e2 : Exp Γ ty_string) :
-      ⟨ γ , μ , δ , stm_assert e1 e2 ⟩ --->
-      ⟨ γ , μ , δ , if eval e1 δ then stm_lit ty_bool true else stm_fail ty_bool (eval e2 δ) ⟩
+  | step_stm_assertk
+      (e1 : Exp Γ ty_bool) (e2 : Exp Γ ty_string) (k : Stm Γ τ) :
+      ⟨ γ , μ , δ , stm_assertk e1 e2 k ⟩ --->
+      ⟨ γ , μ , δ , if eval e1 δ then k else stm_fail τ (eval e2 δ) ⟩
+
   | step_stm_match_list
-      (γ : RegStore) (μ : Memory) (δ : LocalStore Γ) {σ τ : Ty} (e : Exp Γ (ty_list σ)) (alt_nil : Stm Γ τ)
+      {σ : Ty} (e : Exp Γ (ty_list σ)) (alt_nil : Stm Γ τ)
       (xh xt : 𝑿) (alt_cons : Stm (Γ ▻ (xh , σ) ▻ (xt , ty_list σ)) τ) :
       ⟨ γ , μ , δ , stm_match_list e alt_nil xh xt alt_cons ⟩ --->
       ⟨ γ , μ , δ , match eval e δ with
@@ -137,7 +143,7 @@ Module SmallStep
                 end
       ⟩
   | step_stm_match_sum
-      (γ : RegStore) (μ : Memory) (δ : LocalStore Γ) {σinl σinr τ : Ty} (e : Exp Γ (ty_sum σinl σinr))
+      {σinl σinr : Ty} (e : Exp Γ (ty_sum σinl σinr))
       (xinl : 𝑿) (alt_inl : Stm (Γ ▻ (xinl , σinl)) τ)
       (xinr : 𝑿) (alt_inr : Stm (Γ ▻ (xinr , σinr)) τ) :
       ⟨ γ , μ , δ , stm_match_sum e xinl alt_inl xinr alt_inr ⟩ --->
@@ -147,25 +153,23 @@ Module SmallStep
                 end
       ⟩
   | step_stm_match_pair
-      (γ : RegStore) (μ : Memory) (δ : LocalStore Γ) {σ1 σ2 τ : Ty} (e : Exp Γ (ty_prod σ1 σ2)) (xl xr : 𝑿)
+      {σ1 σ2 : Ty} (e : Exp Γ (ty_prod σ1 σ2)) (xl xr : 𝑿)
       (rhs : Stm (Γ ▻ (xl , σ1) ▻ (xr , σ2)) τ) :
       ⟨ γ , μ , δ , stm_match_pair e xl xr rhs ⟩ --->
       ⟨ γ , μ , δ , let (vl , vr) := eval e δ in
                 stm_block (env_snoc (env_snoc env_nil (xl,σ1) vl) (xr,σ2) vr) rhs
       ⟩
   | step_stm_match_enum
-      (γ : RegStore) (μ : Memory) (δ : LocalStore Γ) {E : 𝑬} (e : Exp Γ (ty_enum E)) {τ : Ty}
+      {E : 𝑬} (e : Exp Γ (ty_enum E))
       (alts : forall (K : 𝑬𝑲 E), Stm Γ τ) :
       ⟨ γ , μ , δ , stm_match_enum E e alts ⟩ ---> ⟨ γ , μ , δ , alts (eval e δ) ⟩
   | step_stm_match_tuple
-      (γ : RegStore) (μ : Memory) (δ : LocalStore Γ) {σs : Ctx Ty} {Δ : Ctx (𝑿 * Ty)}
-      (e : Exp Γ (ty_tuple σs)) (p : TuplePat σs Δ)
-      {τ : Ty} (rhs : Stm (ctx_cat Γ Δ) τ) :
+      {Δ σs} (e : Exp Γ (ty_tuple σs)) (p : TuplePat σs Δ) (rhs : Stm (ctx_cat Γ Δ) τ) :
       ⟨ γ , μ , δ , stm_match_tuple e p rhs ⟩ --->
       ⟨ γ , μ , δ , stm_block (tuple_pattern_match p (eval e δ)) rhs ⟩
 
   | step_stm_match_union
-      (γ : RegStore) (μ : Memory) (δ : LocalStore Γ) {U : 𝑼} (e : Exp Γ (ty_union U)) {τ : Ty}
+      {U : 𝑼} (e : Exp Γ (ty_union U))
       (alt__ctx : forall (K : 𝑼𝑲 U), Ctx (𝑿 * Ty))
       (alt__pat : forall (K : 𝑼𝑲 U), Pattern (alt__ctx K) (𝑼𝑲_Ty K))
       (alt__rhs : forall (K : 𝑼𝑲 U), Stm (Γ ▻▻ alt__ctx K) τ) :
@@ -174,45 +178,44 @@ Module SmallStep
                 stm_block (pattern_match (alt__pat K) v) (alt__rhs K)
       ⟩
   | step_stm_match_record
-      (γ : RegStore) (μ : Memory) (δ : LocalStore Γ) {R : 𝑹} {Δ : Ctx (𝑿 * Ty)}
-      (e : Exp Γ (ty_record R)) (p : RecordPat (𝑹𝑭_Ty R) Δ)
-      {τ : Ty} (rhs : Stm (ctx_cat Γ Δ) τ) :
+      {R : 𝑹} {Δ : Ctx (𝑿 * Ty)} (e : Exp Γ (ty_record R))
+      (p : RecordPat (𝑹𝑭_Ty R) Δ) (rhs : Stm (ctx_cat Γ Δ) τ) :
       ⟨ γ , μ , δ , stm_match_record R e p rhs ⟩ --->
       ⟨ γ , μ , δ , stm_block (record_pattern_match p (𝑹_unfold (eval e δ))) rhs ⟩
 
   | step_stm_read_register
-      (γ : RegStore) (μ : Memory) (δ : LocalStore Γ) {σ : Ty} (r : 𝑹𝑬𝑮 σ) :
-      ⟨ γ, μ , δ, stm_read_register r ⟩ ---> ⟨ γ, μ , δ, stm_lit σ (read_register γ r) ⟩
+      (r : 𝑹𝑬𝑮 τ) :
+      ⟨ γ, μ , δ, stm_read_register r ⟩ ---> ⟨ γ, μ , δ, stm_lit τ (read_register γ r) ⟩
   | step_stm_write_register
-      (γ : RegStore) (μ : Memory) (δ : LocalStore Γ) {σ : Ty} (r : 𝑹𝑬𝑮 σ) (e : Exp Γ σ) :
+      (r : 𝑹𝑬𝑮 τ) (e : Exp Γ τ) :
       let v := eval e δ in
-      ⟨ γ , μ , δ, stm_write_register r e ⟩ ---> ⟨ write_register γ r v , μ , δ , stm_lit σ v ⟩
-
+      ⟨ γ , μ , δ, stm_write_register r e ⟩ ---> ⟨ write_register γ r v , μ , δ , stm_lit τ v ⟩
 
   | step_stm_bind_step
-      (γ γ' : RegStore) (μ μ' : Memory) (δ δ' : LocalStore Γ) (σ τ : Ty) (s s' : Stm Γ σ) (k : Lit σ -> Stm Γ τ) :
+      (σ : Ty) (s s' : Stm Γ σ) (k : Lit σ -> Stm Γ τ)
+      (γ' : RegStore) (μ' : Memory) (δ' : LocalStore Γ) :
       ⟨ γ , μ , δ , s ⟩ ---> ⟨ γ', μ' , δ' , s' ⟩ ->
       ⟨ γ , μ , δ , stm_bind s k ⟩ ---> ⟨ γ', μ' , δ' , stm_bind s' k ⟩
   | step_stm_bind_value
-      (γ : RegStore) (μ : Memory) (δ : LocalStore Γ) (σ τ : Ty) (v : Lit σ) (k : Lit σ -> Stm Γ τ) :
+      (σ : Ty) (v : Lit σ) (k : Lit σ -> Stm Γ τ) :
       ⟨ γ , μ , δ , stm_bind (stm_lit σ v) k ⟩ ---> ⟨ γ , μ , δ , k v ⟩
   | step_stm_bind_fail
-      (γ : RegStore) (μ : Memory) (δ : LocalStore Γ) (σ τ : Ty) (s : string) (k : Lit σ -> Stm Γ τ) :
+      (σ : Ty) (s : string) (k : Lit σ -> Stm Γ τ) :
       ⟨ γ , μ , δ , stm_bind (stm_fail σ s) k ⟩ ---> ⟨ γ , μ , δ , stm_fail τ s ⟩
 
-  where "⟨ γ1 , μ1 , δ1 , s1 ⟩ ---> ⟨ γ2 , μ2 , δ2 , s2 ⟩" := (@Step _ _ γ1%env γ2%env μ1%env μ2%env δ1%env δ2%env s1%stm s2%stm).
+  where "⟨ γ1 , μ1 , δ1 , s1 ⟩ ---> ⟨ γ2 , μ2 , δ2 , s2 ⟩" := (@Step _ _ γ1%env μ1%env δ1%env γ2%env μ2%env δ2%env s1%stm s2%stm).
 
   Inductive Steps {Γ : Ctx (𝑿 * Ty)} {σ : Ty} (γ1 : RegStore) (μ1 : Memory) (δ1 : LocalStore Γ) (s1 : Stm Γ σ) : RegStore -> Memory -> LocalStore Γ -> Stm Γ σ -> Prop :=
   | step_refl : Steps γ1 μ1 δ1 s1 γ1 μ1 δ1 s1
   | step_trans {γ2 γ3 : RegStore} {μ2 μ3 : Memory} {δ2 δ3 : LocalStore Γ} {s2 s3 : Stm Γ σ} :
-      Step γ1 γ2 μ1 μ2 δ1 δ2 s1 s2 -> Steps γ2 μ2 δ2 s2 γ3 μ3 δ3 s3 -> Steps γ1 μ1 δ1 s1 γ3 μ3 δ3 s3.
+      Step γ1 μ1 δ1 γ2 μ2 δ2 s1 s2 -> Steps γ2 μ2 δ2 s2 γ3 μ3 δ3 s3 -> Steps γ1 μ1 δ1 s1 γ3 μ3 δ3 s3.
 
   Notation "⟨ γ1 , μ1 , δ1 , s1 ⟩ --->* ⟨ γ2 , μ2 , δ2 , s2 ⟩" := (@Steps _ _ γ1 μ1 δ1 s1 γ2 μ2 δ2 s2).
 
   Inductive StepsN {Γ : Ctx (𝑿 * Ty)} {σ : Ty} (γ1 : RegStore) (μ1 : Memory) (δ1 : LocalStore Γ) (s1 : Stm Γ σ) : nat -> RegStore -> Memory -> LocalStore Γ -> Stm Γ σ -> Prop :=
   | stepsn_refl : StepsN γ1 μ1 δ1 s1 O γ1 μ1 δ1 s1
   | stepsn_trans {γ2 γ3 : RegStore} {μ2 μ3 : Memory} {δ2 δ3 : LocalStore Γ} {s2 s3 : Stm Γ σ} {n} :
-      Step γ1 γ2 μ1 μ2 δ1 δ2 s1 s2 -> StepsN γ2 μ2 δ2 s2 n γ3 μ3 δ3 s3 -> StepsN γ1 μ1 δ1 s1 (S n) γ3 μ3 δ3 s3.
+      Step γ1 μ1 δ1 γ2 μ2 δ2 s1 s2 -> StepsN γ2 μ2 δ2 s2 n γ3 μ3 δ3 s3 -> StepsN γ1 μ1 δ1 s1 (S n) γ3 μ3 δ3 s3.
 
   Notation "⟨ γ1 , μ1 , δ1 , s1 ⟩ ---> n ⟨ γ2 , μ2 , δ2 , s2 ⟩" := (@StepsN _ _ γ1 μ1 δ1 s1 n γ2 μ2 δ2 s2).
 
@@ -236,17 +239,17 @@ Module SmallStep
   Ltac microsail_stm_primitive_step s :=
     first
       [ lazymatch s with
-        | stm_call_frame _ _ _ ?s' => microsail_stm_is_final s'
-        | stm_let _ _ ?s' _        => microsail_stm_is_final s'
-        | stm_block _ ?s'          => microsail_stm_is_final s'
-        | stm_seq ?s' _            => microsail_stm_is_final s'
-        | stm_assign _ ?s'         => microsail_stm_is_final s'
-        | stm_bind ?s' _           => microsail_stm_is_final s'
+        | stm_call_frame _ ?s' => microsail_stm_is_final s'
+        | stm_let _ _ ?s' _    => microsail_stm_is_final s'
+        | stm_block _ ?s'      => microsail_stm_is_final s'
+        | stm_seq ?s' _        => microsail_stm_is_final s'
+        | stm_assign _ ?s'     => microsail_stm_is_final s'
+        | stm_bind ?s' _       => microsail_stm_is_final s'
         end
       | lazymatch head s with
         | @stm_call           => idtac
         | @stm_call_external  => idtac
-        | @stm_assert         => idtac
+        | @stm_assertk        => idtac
         | @stm_fail           => idtac
         | @stm_exp            => idtac
         | @stm_if             => idtac
@@ -279,6 +282,6 @@ Module SmallStep
            tactic should recognize it. *)
         microsail_stm_primitive_step s1'; constructor
       end; fail.
-  Qed.
+    Abort.
 
 End SmallStep.
